Indent in Combi/

theories/Combi/tableau.v
@@ -49,30 +49,31 @@ Open Scope N.
 (** ** Specialization of sorted Lemmas *)
 Section Rows.
 
-  Variable T : inhOrdType.
+Variable T : inhOrdType.
 
-  Implicit Type l : T.
-  Implicit Type r : seq T.
+Implicit Type l : T.
+Implicit Type r : seq T.
 
-  Notation is_row r := (sorted leqX_op r).
+Notation is_row r := (sorted leqX_op r).
 
-  Definition is_row1P Z r := sorted1P Z leqX_op r.
-  Definition is_rowP Z r := sortedP Z (@leqX_trans T) (@leqXnn T) r.
-  Definition is_row_cons := sorted_cons (@leqXnn T).
-  Definition is_row_consK := sorted_consK (R := @leqX_op T).
-  Definition is_row_rcons := sorted_rcons (R := @leqX_op T).
-  Definition is_row_rconsK := sorted_rconsK (R := @leqX_op T).
-  Definition is_row_last := sorted_last (@leqXnn T).
-  Definition is_row_take := sorted_take (R := @leqX_op T).
-  Definition is_row_drop := sorted_drop (R := @leqX_op T).
-  Definition is_row_catL := sorted_catL (R := @leqX_op T).
-  Definition is_row_catR := sorted_catR (R := @leqX_op T).
-  Definition head_leq_last_row := head_leq_last_sorted (@leqX_trans T) (@leqXnn T).
-  Lemma row_lt_by_pos Z r p q:
-    is_row r -> p < size r -> q < size r -> nth Z r p <A nth Z r q -> p < q.
-  Proof using .
-    rewrite /ltnX_op. apply: (sorted_lt_by_pos (@leqX_trans T) (@leqXnn T) (@anti_leqX T)). 
-  Qed.
+Definition is_row1P Z r := sorted1P Z leqX_op r.
+Definition is_rowP Z r := sortedP Z (@leqX_trans T) (@leqXnn T) r.
+Definition is_row_cons := sorted_cons (@leqXnn T).
+Definition is_row_consK := sorted_consK (R := @leqX_op T).
+Definition is_row_rcons := sorted_rcons (R := @leqX_op T).
+Definition is_row_rconsK := sorted_rconsK (R := @leqX_op T).
+Definition is_row_last := sorted_last (@leqXnn T).
+Definition is_row_take := sorted_take (R := @leqX_op T).
+Definition is_row_drop := sorted_drop (R := @leqX_op T).
+Definition is_row_catL := sorted_catL (R := @leqX_op T).
+Definition is_row_catR := sorted_catR (R := @leqX_op T).
+Definition head_leq_last_row := head_leq_last_sorted (@leqX_trans T) (@leqXnn T).
+Lemma row_lt_by_pos Z r p q:
+  is_row r -> p < size r -> q < size r -> nth Z r p <A nth Z r q -> p < q.
+Proof using.
+rewrite /ltnX_op.
+by apply: (sorted_lt_by_pos (@leqX_trans T) (@leqXnn T) (@anti_leqX T)). 
+Qed.
 
 End Rows.
 
@@ -81,85 +82,88 @@ Notation is_row r := (sorted leqX_op r).
 (** ** Dominance order for rows *)
 Section Dominate.
 
-  Variable T : inhOrdType.
-  Notation Z := (inhabitant T).
+Variable T : inhOrdType.
+Notation Z := (inhabitant T).
 
-  Implicit Type l : T.
-  Implicit Type r u v : seq T.
+Implicit Type l : T.
+Implicit Type r u v : seq T.
 
 Lemma is_row_set_nth l r pos :
   is_row r -> l <A nth l r pos ->
   (forall n : nat, l <A nth l r n -> pos <= n) -> is_row (set_nth l r pos l).
-Proof using .
-  move=> /is_row1P Hrow Hl Hmin. apply/(is_row1P l) => i.
-  rewrite (lock (i.+1)) !nth_set_nth /=; unlock.
-  case: (ltnP pos (size r)) Hl => [Hpos Hl |HH]; last by rewrite (nth_default l HH) ltnXnn.
-  rewrite size_set_nth maxnC /maxn; move: Hpos; rewrite leqNgt; move/negbTE => -> Hi1lt.
-  case eqP => Hipos; case eqP => Hi1pos.
-  - exact: leqXnn.
-  - apply: ltnXW; apply: (ltnX_leqX_trans Hl); rewrite -Hipos; exact: Hrow.
-  - move: {Hmin} (contra (Hmin i)); rewrite -leqXNgtnX -ltnNge; apply.
-    by rewrite Hi1pos leqnn.
-  - exact: Hrow.
+Proof using.
+move=> /is_row1P Hrow Hl Hmin. apply/(is_row1P l) => i.
+rewrite (lock (i.+1)) !nth_set_nth /=; unlock.
+case: (ltnP pos (size r)) Hl => [Hpos Hl |HH]; first last.
+  by rewrite (nth_default l HH) ltnXnn.
+rewrite size_set_nth maxnC /maxn.
+move: Hpos; rewrite leqNgt; move/negbTE => -> Hi1lt.
+case eqP => Hipos; case eqP => Hi1pos.
+- exact: leqXnn.
+- by apply: ltnXW; apply: (ltnX_leqX_trans Hl); rewrite -Hipos; apply: Hrow.
+- move: {Hmin} (contra (Hmin i)); rewrite -leqXNgtnX -ltnNge; apply.
+  by rewrite Hi1pos leqnn.
+- exact: Hrow.
 Qed.
 
-  Definition dominate u v :=
-    ((size u) <= (size v)) && (all (fun i => nth Z u i >A nth Z v i) (iota 0 (size u))).
+Definition dominate u v :=
+  ((size u) <= (size v)) &&
+   (all (fun i => nth Z u i >A nth Z v i) (iota 0 (size u))).
 
-  Lemma dominateP u v :
-    reflect ((size u) <= (size v) /\ forall i, i < size u -> nth Z u i >A nth Z v i)
-            (dominate u v).
-  Proof using .
-    rewrite /dominate /mkseq ; apply/(iffP idP).
-    - move=> /andP [] Hsz /allP Hall; split; first by exact Hsz.
-      move=> i Hi; apply: Hall; by rewrite mem_iota add0n.
-    - move=> [] -> /= H; apply/allP => i; rewrite mem_iota add0n; exact: H.
-  Qed.
+Lemma dominateP u v :
+  reflect ((size u) <= (size v) /\ forall i, i < size u -> nth Z u i >A nth Z v i)
+          (dominate u v).
+Proof using.
+rewrite /dominate /mkseq ; apply/(iffP idP).
+- move=> /andP [] Hsz /allP Hall; split; first exact Hsz.
+  by move=> i Hi; apply: Hall; rewrite mem_iota add0n.
+- by move=> [] -> /= H; apply/allP => i; rewrite mem_iota add0n; apply: H.
+Qed.
 
-  Lemma dominate_nil u : dominate [::] u.
-  Proof using . apply/dominateP => /=; by split. Qed.
+Lemma dominate_nil u : dominate [::] u.
+Proof using. by apply/dominateP. Qed.
 
-  Lemma dominate_trans r0 r1 r2 :
-    dominate r0 r1 -> dominate r1 r2 -> dominate r0 r2.
-  Proof using .
-    move=> /dominateP [] Hsz0 Hdom0 /dominateP [] Hsz1 Hdom1.
-    apply/dominateP; split; first exact: (leq_trans Hsz0 Hsz1).
-    move => i Hi.
-    apply (ltnX_trans (Hdom1 i (leq_trans Hi Hsz0))).
-    exact: Hdom0.
-  Qed.
+Lemma dominate_trans r0 r1 r2 :
+  dominate r0 r1 -> dominate r1 r2 -> dominate r0 r2.
+Proof using.
+move=> /dominateP [] Hsz0 Hdom0 /dominateP [] Hsz1 Hdom1.
+apply/dominateP; split; first exact: (leq_trans Hsz0 Hsz1).
+move => i Hi.
+apply (ltnX_trans (Hdom1 i (leq_trans Hi Hsz0))).
+exact: Hdom0.
+Qed.
 
-  Lemma dominate_rcons v u l : dominate u v -> dominate u (rcons v l).
-  Proof using .
-    move /dominateP => [] Hsz Hlt.
-    apply/dominateP; split => [|i Hi]; first by rewrite size_rcons; apply: leqW.
-    move/(_ _ Hi) : Hlt; rewrite nth_rcons.
-    case: (ltnP i (size v)) => //= /(leq_trans Hsz)/leq_ltn_trans/(_ Hi).
-    by rewrite ltnn.
-  Qed.
+Lemma dominate_rcons v u l : dominate u v -> dominate u (rcons v l).
+Proof using.
+move/dominateP => [] Hsz Hlt.
+apply/dominateP; split => [|i Hi]; first by rewrite size_rcons; apply: leqW.
+move/(_ _ Hi) : Hlt; rewrite nth_rcons.
+case: (ltnP i (size v)) => //= /(leq_trans Hsz)/leq_ltn_trans/(_ Hi).
+by rewrite ltnn.
+Qed.
 
-  Lemma dominate_rconsK u v l :
-    size u <= size v -> dominate u (rcons v l) -> dominate u v.
-  Proof using .
-    move=> Hsz /dominateP [] _ Hlt.
-    apply/dominateP; split => [|i Hi]; first exact Hsz.
-    move/(_ _ Hi) : Hlt; by rewrite nth_rcons (leq_trans Hi Hsz).
-  Qed.
+Lemma dominate_rconsK u v l :
+  size u <= size v -> dominate u (rcons v l) -> dominate u v.
+Proof using.
+move=> Hsz /dominateP [] _ Hlt.
+apply/dominateP; split => [|i Hi]; first exact Hsz.
+by move/(_ _ Hi) : Hlt; rewrite nth_rcons (leq_trans Hi Hsz).
+Qed.
 
-  Lemma dominate_head u v : u != [::] -> dominate u v -> head Z v <A head Z u.
-  Proof using .
-    move=> Hu /dominateP []; case: u Hu => [//=|u0 u _]; case: v => [|v0 v _] /=.
-    - by rewrite ltn0.
-    - move=> Hdom; exact: (Hdom 0 (ltn0Sn _)).
-  Qed.
+Lemma dominate_head u v : u != [::] -> dominate u v -> head Z v <A head Z u.
+Proof using.
+move=> Hu /dominateP []; case: u Hu => [//=|u0 u _]; case: v => [|v0 v _] /=.
+- by rewrite ltn0.
+- by move=> Hdom; apply: (Hdom 0 (ltn0Sn _)).
+Qed.
 
-  Lemma dominate_tl a u b v :
-    dominate (a :: u) (b :: v) -> dominate u v.
-  Proof using .
-    move=> /dominateP [] /=; rewrite ltnS => Hsize Hdom.
-    apply/dominateP; split; first exact Hsize.
-    move=> i Hi; exact: (Hdom i.+1 Hi).
-  Qed.
+Lemma dominate_tl a u b v :
+  dominate (a :: u) (b :: v) -> dominate u v.
+Proof using.
+move=> /dominateP [] /=; rewrite ltnS => Hsize Hdom.
+apply/dominateP; split; first exact Hsize.
+  by move=> i Hi; apply: (Hdom i.+1 Hi).
+Qed.
 
 End Dominate.
 
@@ -167,231 +171,237 @@ End Dominate.
 (** * Tableaux : definition and basic properties *)
 Section Tableau.
 
-  Variable T : inhOrdType.
-  Notation Z := (inhabitant T).
+Variable T : inhOrdType.
+Notation Z := (inhabitant T).
 
-  Implicit Type l : T.
-  Implicit Type r w : seq T.
-  Implicit Type t : seq (seq T).
+Implicit Type l : T.
+Implicit Type r w : seq T.
+Implicit Type t : seq (seq T).
 
-  Fixpoint is_tableau t :=
-    if t is t0 :: t'
-    then [&& (t0 != [::]), is_row t0, dominate (head [::] t') t0 & is_tableau t']
-    else true.
+Fixpoint is_tableau t :=
+  if t is t0 :: t'
+  then [&& (t0 != [::]), is_row t0, dominate (head [::] t') t0 & is_tableau t']
+  else true.
 
-  Definition get_tab (t : seq (seq T)) (r c : nat) :=
-    nth (inhabitant T) (nth [::] t r) c.
+Definition get_tab (t : seq (seq T)) (r c : nat) :=
+  nth (inhabitant T) (nth [::] t r) c.
 
-  Definition to_word t := flatten (rev t).
+Definition to_word t := flatten (rev t).
 
-  (* Shape is defined in seq.v *)
-  (* Definition shape t := map size t. *)
+(* Shape is defined in seq.v *)
+(* Definition shape t := map size t. *)
 
-  Lemma is_tableauP t : reflect
+Lemma is_tableauP t :
+  reflect
     [/\ forall i, i < size t -> (nth [::] t i) != [::], (* forbid empty lines *)
-     forall i, is_row (nth [::] t i) &
-     forall i j, i < j -> dominate (nth [::] t j) (nth [::] t i)]
+        forall i, is_row (nth [::] t i) &
+        forall i j, i < j -> dominate (nth [::] t j) (nth [::] t i)]
     (is_tableau t).
-  Proof using .
-    apply (iffP idP).
-    - elim: t => [_ | t0 t IHt] /=.
-        split=> i //=; first by rewrite nth_default.
-        move=> j; by rewrite !nth_default.
-      move=> /and4P [] Ht0 Hrow0 Hdom0 /IHt {IHt} [] Hnnil Hrow Hdom.
-      split; try by case.
-      case=> [| i] [| j] //=.
-      + case: j => [|j] _; first by rewrite nth0.
-        apply: (dominate_trans _ Hdom0).
-        rewrite -nth0; exact: Hdom.
-      + rewrite ltnS; exact: Hdom.
-    - elim: t => [| t0 t IHt] //= [] Hnnil Hrow Hdom.
-      apply/and4P; split.
-      + exact: (Hnnil 0).
-      + exact: (Hrow 0).
-      + move: Hdom; case t => [| t1 tt] //= H.
-        rewrite -/(nth [::] (t0 :: t1 :: tt) 0) -/(nth [::] (t0 :: t1 :: tt) 1).
-        exact: H.
-      + apply IHt; split => [i H | i | i j H].
-        * exact: (Hnnil i.+1).
-        * exact: (Hrow i.+1).
-        * exact: (Hdom i.+1 j.+1).
-  Qed.
+Proof using.
+apply (iffP idP).
+- elim: t => [_ | t0 t IHt] /=.
+    split=> i //=; first by rewrite nth_default.
+    by move=> j; rewrite !nth_default.
+  move=> /and4P [] Ht0 Hrow0 Hdom0 /IHt {IHt} [] Hnnil Hrow Hdom.
+  split; try by case.
+  case=> [| i] [| j] //=.
+  + case: j => [|j] _; first by rewrite nth0.
+    apply: (dominate_trans _ Hdom0).
+    by rewrite -nth0; apply: Hdom.
+  + by rewrite ltnS; apply: Hdom.
+- elim: t => [| t0 t IHt] //= [] Hnnil Hrow Hdom.
+  apply/and4P; split.
+  + exact: (Hnnil 0).
+  + exact: (Hrow 0).
+  + move: Hdom; case t => [| t1 tt] //= H.
+    rewrite -/(nth [::] (t0 :: t1 :: tt) 0) -/(nth [::] (t0 :: t1 :: tt) 1).
+    exact: H.
+  + apply IHt; split => [i H | i | i j H].
+    * exact: (Hnnil i.+1).
+    * exact: (Hrow i.+1).
+    * exact: (Hdom i.+1 j.+1).
+Qed.
 
-  Lemma get_tab_default t (r c : nat) : ~~ is_in_shape (shape t) r c -> get_tab t r c = Z.
-  Proof using . rewrite /is_in_shape /get_tab -leqNgt nth_shape => Hc; exact: nth_default. Qed.
+Lemma get_tab_default t (r c : nat) :
+  ~~ is_in_shape (shape t) r c -> get_tab t r c = Z.
+Proof using.
+rewrite /is_in_shape /get_tab -leqNgt nth_shape => Hc.
+exact: nth_default.
+Qed.
 
-  Lemma to_word_cons r t : to_word (r :: t) = to_word t ++ r.
-  Proof using . by rewrite /to_word rev_cons flatten_rcons. Qed.
-  Lemma to_word_rcons r t : to_word (rcons t r) = r ++ to_word t.
-  Proof using . by rewrite /to_word rev_rcons /=. Qed.
+Lemma to_word_cons r t : to_word (r :: t) = to_word t ++ r.
+Proof using. by rewrite /to_word rev_cons flatten_rcons. Qed.
+Lemma to_word_rcons r t : to_word (rcons t r) = r ++ to_word t.
+Proof using. by rewrite /to_word rev_rcons /=. Qed.
 
-  Lemma mem_to_word t (r c : nat) :
-    is_in_shape (shape t) r c -> (get_tab t r c) \in (to_word t).
-  Proof using .
-    rewrite /is_in_shape /get_tab.
-    elim: t r c => [//= | t0 t IHt] /= r c; first by rewrite nth_default.
-    rewrite to_word_cons mem_cat => H.
-    case: r H => [/mem_nth ->| r] /=; first by rewrite orbT.
-    by move/IHt ->.
-  Qed.
+Lemma mem_to_word t (r c : nat) :
+  is_in_shape (shape t) r c -> (get_tab t r c) \in (to_word t).
+Proof using.
+rewrite /is_in_shape /get_tab.
+elim: t r c => [//= | t0 t IHt] /= r c; first by rewrite nth_default.
+rewrite to_word_cons mem_cat => H.
+case: r H => [/mem_nth ->| r] /=; first by rewrite orbT.
+by move/IHt ->.
+Qed.
 
-  Lemma to_wordK t : rev (reshape (rev (shape t)) (to_word t)) = t.
-  Proof using . by rewrite -shape_rev /to_word flattenK revK. Qed.
+Lemma to_wordK t : rev (reshape (rev (shape t)) (to_word t)) = t.
+Proof using. by rewrite -shape_rev /to_word flattenK revK. Qed.
 
-  Lemma tableau_is_row r t : is_tableau (r :: t) -> is_row r.
-  Proof using . by move=> /= /and4P []. Qed.
+Lemma tableau_is_row r t : is_tableau (r :: t) -> is_row r.
+Proof using. by move=> /= /and4P []. Qed.
 
-  Lemma  is_tableau_rconsK t (tn : seq T) :
-    is_tableau (rcons t tn) -> is_tableau t.
-  Proof using .
-    elim: t => [//= | t0 t IHt] /= /and4P [] -> -> Hdom /IHt -> /= {IHt}.
-    case: t Hdom => [//=| t1 t]; by rewrite rcons_cons /= => ->.
-  Qed.
+Lemma  is_tableau_rconsK t (tn : seq T) :
+  is_tableau (rcons t tn) -> is_tableau t.
+Proof using.
+elim: t => [//= | t0 t IHt] /= /and4P [] -> -> Hdom /IHt -> /= {IHt}.
+by case: t Hdom => [//=| t1 t]; rewrite rcons_cons /= => ->.
+Qed.
 
-  Lemma is_tableau_catl t1 t2 :
-    is_tableau (t1 ++ t2) -> is_tableau t1.
-  Proof.
-    elim: t1 => [//= | t t1 IHt1] /= /and4P [] -> -> /= Hdom /IHt1 {IHt1} ->.
-    rewrite andbT; by case: t1 Hdom => [//= | r1 t1].
-  Qed.
+Lemma is_tableau_catl t1 t2 :
+  is_tableau (t1 ++ t2) -> is_tableau t1.
+Proof.
+elim: t1 => [//= | t t1 IHt1] /= /and4P [] -> -> /= Hdom /IHt1 {IHt1} ->.
+by rewrite andbT; case: t1 Hdom => [//= | r1 t1].
+Qed.
 
-  Lemma is_tableau_catr t1 t2 :
-    is_tableau (t1 ++ t2) -> is_tableau t2.
-  Proof. by elim: t1 => [//= | r t1 IHt1] /= /and4P [] _ _ _. Qed.
+Lemma is_tableau_catr t1 t2 :
+  is_tableau (t1 ++ t2) -> is_tableau t2.
+Proof. by elim: t1 => [//= | r t1 IHt1] /= /and4P [] _ _ _. Qed.
 
-  Lemma is_part_sht t : is_tableau t -> is_part (shape t).
-  Proof using .
-    elim: t => [//= | t0 t IHt] /= /and4P [] Ht0 _ /dominateP [] Hdom _ Htab.
-    rewrite (IHt Htab) andbT {IHt Htab} /shape.
-    case: t Hdom => //=; by case: t0 Ht0.
-  Qed.
+Lemma is_part_sht t : is_tableau t -> is_part (shape t).
+Proof using.
+elim: t => [//= | t0 t IHt] /= /and4P [] Ht0 _ /dominateP [] Hdom _ Htab.
+rewrite (IHt Htab) andbT {IHt Htab} /shape.
+by case: t Hdom => //=; case: t0 Ht0.
+Qed.
 
-  Lemma tab_eqP p q :
-    is_tableau p -> is_tableau q -> reflect (forall i, nth [::] p i = nth [::] q i) (p == q).
-  Proof using .
-    move=> Hp Hq.
-    apply (iffP idP) => [/eqP -> //| H].
-    have Hnth t i : nth 0 (shape t) i = size (nth [::] t i).
-      case: (ltnP i (size t)) => Hi.
-      - by rewrite /shape (nth_map [::] _ _ Hi).
-      - by rewrite !nth_default // size_map.
-    have Hsz : size p = size q.
-      rewrite -!(size_map size); congr (size _).
-      apply/eqP/(part_eqP (is_part_sht Hp) (is_part_sht Hq)) => i.
-      by rewrite !Hnth H.
-    apply/eqP; by apply (eq_from_nth (x0 := [::]) Hsz) => i _.
-  Qed.
+Lemma tab_eqP p q :
+  is_tableau p -> is_tableau q ->
+  reflect (forall i, nth [::] p i = nth [::] q i) (p == q).
+Proof using.
+move=> Hp Hq.
+apply (iffP idP) => [/eqP -> //| H].
+have Hnth t i : nth 0 (shape t) i = size (nth [::] t i).
+  case: (ltnP i (size t)) => Hi.
+  - by rewrite /shape (nth_map [::] _ _ Hi).
+  - by rewrite !nth_default // size_map.
+have Hsz : size p = size q.
+  rewrite -!(size_map size); congr (size _).
+  apply/eqP/(part_eqP (is_part_sht Hp) (is_part_sht Hq)) => i.
+  by rewrite !Hnth H.
+by apply/eqP; apply (eq_from_nth (x0 := [::]) Hsz) => i _.
+Qed.
 
-  Lemma is_tableau_sorted_dominate (t : seq (seq T)) :
-    is_tableau t =
-    [&& is_part (shape t),
-     all (sorted leqX_op) t &
-     sorted (fun x y => dominate y x) t].
-  Proof using .
-    apply/idP/idP; elim: t => [//= | t0 t IHt].
-    - move=> /=/and4P [] Hnnil Hrow0 Hdom /IHt /and3P [] Hpart Hall Hsort.
-      rewrite Hpart Hrow0 Hall {Hpart Hrow0 Hall IHt} !andbT /=; apply/andP; split.
-      + case: t Hdom {Hsort} => [_ | t1 t] /=; first by case: t0 Hnnil.
-        by move => /dominateP [].
-      + by case: t Hdom Hsort => [//=| t1 t]/= -> ->.
-    - move=>/and3P [] Hpart.
-      have:= part_head_non0 Hpart.
-      rewrite [head _ _]/= [all _ _]/= [is_tableau _]/=.
-      move=> /nilP /eqP -> /andP [] -> Hall Hsort /=.
-      apply/andP; split.
-      + by case: t Hsort {Hpart Hall IHt} => [//= | t1 t] /= /andP [].
-      + apply: IHt; rewrite (is_part_consK Hpart) Hall /=.
-        exact: (sorted_consK Hsort).
-  Qed.
+Lemma is_tableau_sorted_dominate (t : seq (seq T)) :
+  is_tableau t =
+  [&& is_part (shape t),
+   all (sorted leqX_op) t &
+   sorted (fun x y => dominate y x) t].
+Proof using.
+apply/idP/idP; elim: t => [//= | t0 t IHt].
+- move=> /=/and4P [] Hnnil Hrow0 Hdom /IHt /and3P [] Hpart Hall Hsort.
+  rewrite Hpart Hrow0 Hall {Hpart Hrow0 Hall IHt} !andbT /=; apply/andP; split.
+  + case: t Hdom {Hsort} => [_ | t1 t] /=; first by case: t0 Hnnil.
+    by move => /dominateP [].
+  + by case: t Hdom Hsort => [//=| t1 t]/= -> ->.
+- move=>/and3P [] Hpart.
+  have:= part_head_non0 Hpart.
+  rewrite [head _ _]/= [all _ _]/= [is_tableau _]/=.
+  move=> /nilP /eqP -> /andP [] -> Hall Hsort /=.
+  apply/andP; split.
+  + by case: t Hsort {Hpart Hall IHt} => [//= | t1 t] /= /andP [].
+  + apply: IHt; rewrite (is_part_consK Hpart) Hall /=.
+    exact: (sorted_consK Hsort).
+Qed.
 
-  Lemma is_tableau_getP (t : seq (seq T)) :
-    reflect
-      [/\ is_part (shape t),
-       (forall (r c : nat), is_in_shape (shape t) r c.+1 ->
-                    get_tab t r c <=A get_tab t r c.+1) &
-       (forall (r c : nat), is_in_shape (shape t) r.+1 c ->
-                    get_tab t r c <A get_tab t r.+1 c)]
-      (is_tableau t).
-  Proof using .
-    apply/(iffP idP).
-    - move=> Htab; split.
-      + exact: is_part_sht.
-      + rewrite /is_in_shape /get_tab => r c Hrc.
-        move: Htab => /is_tableauP [] _ Hrow _.
-        apply: (is_row1P _ _ (Hrow r)); by rewrite -nth_shape.
-      + rewrite /is_in_shape /get_tab => r c Hrc.
-        move: Htab => /is_tableauP [] _ _ Hdom.
-        have := dominateP _ _ (Hdom _ _ (ltnSn r)) => [] [] _; apply.
-        by rewrite -nth_shape.
-    - move=> [] Hpart Hrow Hcol.
-      apply/is_tableauP; split.
-      + move=> i Hi.
-        have:= nth_part_non0 Hpart; rewrite size_map => H.
-        have {H} := H _ Hi.
-        apply contra => /eqP.
-        by rewrite nth_shape => ->.
-      + move=> r; apply/(is_row1P (inhabitant T)) => c.
-        rewrite -nth_shape => /Hrow; by apply.
-      + move=> i j Hij; case: (ltnP j (size t)) => Hjr.
-        * have H : i < j < size t by rewrite Hij Hjr.
-          have Htrans : transitive (fun x : seq T => (@dominate T)^~ x).
-            move=> a b c /= Hab Hca; exact: dominate_trans Hca Hab.
-          move: i j H {Hij Hjr}; rewrite (incr_equiv [::] Htrans t) => i Hi.
-          apply/dominateP; rewrite -!nth_shape.
-          split; first by have:= is_partP _ Hpart => [] [] _; apply.
-          move=> j; by rewrite -/(is_in_shape _ _ _) -!/(get_tab _ _ _) => /Hcol ->.
-        * rewrite (nth_default _ Hjr); exact: dominate_nil.
-  Qed.
+Lemma is_tableau_getP (t : seq (seq T)) :
+  reflect
+    [/\ is_part (shape t),
+     (forall (r c : nat), is_in_shape (shape t) r c.+1 ->
+                          get_tab t r c <=A get_tab t r c.+1) &
+     (forall (r c : nat), is_in_shape (shape t) r.+1 c ->
+                          get_tab t r c <A get_tab t r.+1 c)]
+    (is_tableau t).
+Proof using.
+apply/(iffP idP).
+- move=> Htab; split.
+  + exact: is_part_sht.
+  + rewrite /is_in_shape /get_tab => r c Hrc.
+    move: Htab => /is_tableauP [] _ Hrow _.
+    by apply: (is_row1P _ _ (Hrow r)); rewrite -nth_shape.
+  + rewrite /is_in_shape /get_tab => r c Hrc.
+    move: Htab => /is_tableauP [] _ _ Hdom.
+    have := dominateP _ _ (Hdom _ _ (ltnSn r)) => [] [] _; apply.
+    by rewrite -nth_shape.
+- move=> [] Hpart Hrow Hcol.
+  apply/is_tableauP; split.
+  + move=> i Hi.
+    have:= nth_part_non0 Hpart; rewrite size_map => H.
+    have {H} := H _ Hi.
+    apply contra => /eqP.
+    by rewrite nth_shape => ->.
+  + move=> r; apply/(is_row1P (inhabitant T)) => c.
+    by rewrite -nth_shape => /Hrow; apply.
+  + move=> i j Hij; case: (ltnP j (size t)) => Hjr.
+    * have H : i < j < size t by rewrite Hij Hjr.
+      have Htrans : transitive (fun x : seq T => (@dominate T)^~ x).
+        by move=> a b c /= Hab Hca; apply: dominate_trans Hca Hab.
+      move: i j H {Hij Hjr}; rewrite (incr_equiv [::] Htrans t) => i Hi.
+      apply/dominateP; rewrite -!nth_shape.
+      split; first by have:= is_partP _ Hpart => [] [] _; apply.
+      by move=> j; rewrite -/(is_in_shape _ _ _) -!/(get_tab _ _ _) => /Hcol ->.
+    * by rewrite (nth_default _ Hjr); apply: dominate_nil.
+Qed.
 
 Lemma filter_gtnX_row r n :
   is_row r -> filter (gtnX n) r = take (count (gtnX n) r) r.
-Proof using .
-  elim: r => [//= | r0 r IHr] Hrow /=.
-  case: (ltnXP r0 n) => Hr0.
-  - by rewrite add1n (IHr (is_row_consK Hrow)).
-  - rewrite add0n; have Hcount : count (gtnX n) r = 0.
-      elim: r r0 Hr0 Hrow {IHr} => [//= | r1 r /= IHr] r0 Hr0 /andP [] Hr0r1 Hpath.
-      have Hr1 := leqX_trans Hr0 Hr0r1.
-      by rewrite ltnXNgeqX Hr1 (IHr r1 Hr1 Hpath).
-    rewrite Hcount.
-    by apply/nilP; rewrite /nilp size_filter Hcount.
+Proof using.
+elim: r => [//= | r0 r IHr] Hrow /=.
+case: (ltnXP r0 n) => Hr0.
+- by rewrite add1n (IHr (is_row_consK Hrow)).
+- rewrite add0n; have Hcount : count (gtnX n) r = 0.
+  elim: r r0 Hr0 Hrow {IHr} => [//= | r1 r /= IHr] r0 Hr0 /andP [] Hr0r1 Hpath.
+  have Hr1 := leqX_trans Hr0 Hr0r1.
+    by rewrite ltnXNgeqX Hr1 (IHr r1 Hr1 Hpath).
+  rewrite Hcount.
+  by apply/nilP; rewrite /nilp size_filter Hcount.
 Qed.
 
 Lemma count_gtnX_dominate r1 r0 n :
   dominate r1 r0 -> (count (gtnX n) r1) <= (count (gtnX n) r0).
-Proof using .
-  move=> /dominateP [] Hsz Hdom.
-  rewrite -[r0](mkseq_nth Z) -[r1](mkseq_nth Z) /mkseq !count_map.
-  rewrite -(subnKC Hsz).
-  rewrite iota_add count_cat.
-  set s0 := (X in X + _).
-  apply (@leq_trans s0); last exact: leq_addr.
-  rewrite /s0 {s0} -!size_filter.
-  set f1 := (X in filter X ); set f0 := (X in _ <= size (filter X _)).
-  rewrite (eq_in_filter (a1 := f1) (a2 := predI f1 (gtn (size r1)))); first last.
-    move=> i; rewrite mem_iota /= add0n => ->; by rewrite andbT.
-  rewrite (eq_in_filter (a1 := f0) (a2 := predI f0 (gtn (size r1)))); first last.
-    move=> i; rewrite mem_iota /= add0n => ->; by rewrite andbT.
-  rewrite !size_filter; apply sub_count => i /=.
-  rewrite /f1 /f0 {f1 f0} /= => /andP [] Hn Hi.
-  rewrite Hi andbT.
-  exact: (ltnX_trans (Hdom i Hi) Hn).
+Proof using.
+move=> /dominateP [] Hsz Hdom.
+rewrite -[r0](mkseq_nth Z) -[r1](mkseq_nth Z) /mkseq !count_map.
+rewrite -(subnKC Hsz).
+rewrite iota_add count_cat.
+set s0 := (X in X + _).
+apply (@leq_trans s0); last exact: leq_addr.
+rewrite /s0 {s0} -!size_filter.
+set f1 := (X in filter X ); set f0 := (X in _ <= size (filter X _)).
+rewrite (eq_in_filter (a1 := f1) (a2 := predI f1 (gtn (size r1)))); first last.
+  by move=> i; rewrite mem_iota /= add0n => ->; rewrite andbT.
+rewrite (eq_in_filter (a1 := f0) (a2 := predI f0 (gtn (size r1)))); first last.
+  by move=> i; rewrite mem_iota /= add0n => ->; rewrite andbT.
+rewrite !size_filter; apply sub_count => i /=.
+rewrite /f1 /f0 {f1 f0} /= => /andP [] Hn Hi.
+rewrite Hi andbT.
+exact: ltnX_trans (Hdom i Hi) Hn.
 Qed.
 
 Lemma filter_gtnX_dominate r1 r0 n :
-    is_row r0 -> is_row r1 -> dominate r1 r0 ->
-    dominate (filter (gtnX n) r1) (filter (gtnX n) r0).
-Proof using .
-  move=> Hrow0 Hrow1 Hdom.
-  have Hsize := count_gtnX_dominate n Hdom.
-  move: Hdom => /dominateP [] Hsz Hdom.
-  apply/dominateP; rewrite !size_filter.
-  split; first exact Hsize.
-  move=> i Hi.
-  rewrite (filter_gtnX_row _ Hrow0) (filter_gtnX_row _ Hrow1) !nth_take.
-  - apply Hdom; apply (leq_trans Hi); exact: count_size.
-  - exact: Hi.
-  - exact: (leq_trans Hi).
+  is_row r0 -> is_row r1 -> dominate r1 r0 ->
+  dominate (filter (gtnX n) r1) (filter (gtnX n) r0).
+Proof using.
+move=> Hrow0 Hrow1 Hdom.
+have Hsize := count_gtnX_dominate n Hdom.
+move: Hdom => /dominateP [] Hsz Hdom.
+apply/dominateP; rewrite !size_filter.
+split; first exact Hsize.
+move=> i Hi.
+rewrite (filter_gtnX_row _ Hrow0) (filter_gtnX_row _ Hrow1) !nth_take.
+- by apply Hdom; apply (leq_trans Hi); apply: count_size.
+- exact: Hi.
+- exact: (leq_trans Hi).
 Qed.
 
 Definition filter_gtnX_tab n :=
@@ -399,56 +409,56 @@ Definition filter_gtnX_tab n :=
                                    [seq [seq x <- i | gtnX n x] | i <- t]].
 
 Lemma to_word_filter_nnil t : to_word (filter (fun r => r != [::]) t) = to_word t.
-Proof using .
-  elim: t => [//= | t0 t IHt] /=.
-  rewrite to_word_cons -IHt.
-  case: (altP (t0 =P [::])) => [-> | _] /=; first by rewrite cats0.
-  by rewrite to_word_cons.
+Proof using.
+elim: t => [//= | t0 t IHt] /=.
+rewrite to_word_cons -IHt.
+case: (altP (t0 =P [::])) => [-> | _] /=; first by rewrite cats0.
+by rewrite to_word_cons.
 Qed.
 
 Lemma filter_to_word t p : filter p (to_word t) = to_word (map (filter p) t).
-Proof using .
-    elim: t => [//= | t0 t IHt] /=.
-    by rewrite !to_word_cons -IHt filter_cat.
+Proof using.
+elim: t => [//= | t0 t IHt] /=.
+by rewrite !to_word_cons -IHt filter_cat.
 Qed.
 
 Lemma head_filter_gtnX_tab n t :
   is_tableau t ->
   head [::] (filter_gtnX_tab n t) = [seq x <- head [::] t | x <A n].
-Proof using .
-  elim: t => [//= | t0 t /= IHt] /and4P [] Hnnil0 Hrow0 Hdom Htab.
-  case: (altP ([seq x <- t0 | x <A n] =P [::])) => Ht0 //=.
-  rewrite (IHt Htab) Ht0 {IHt}.
-  case: t Hdom Htab => [//= | t1 t] /= Hdom /and3P [] Hnnil1 Hrow1 _.
-  have /dominateP := filter_gtnX_dominate n Hrow0 Hrow1 Hdom => [] [].
-  by rewrite Ht0 /= leqn0 => /nilP ->.
+Proof using.
+elim: t => [//= | t0 t /= IHt] /and4P [] Hnnil0 Hrow0 Hdom Htab.
+case: (altP ([seq x <- t0 | x <A n] =P [::])) => Ht0 //=.
+rewrite (IHt Htab) Ht0 {IHt}.
+case: t Hdom Htab => [//= | t1 t] /= Hdom /and3P [] Hnnil1 Hrow1 _.
+have /dominateP := filter_gtnX_dominate n Hrow0 Hrow1 Hdom => [] [].
+by rewrite Ht0 /= leqn0 => /nilP ->.
 Qed.
 
 Lemma is_tableau_filter_gtnX t n : is_tableau t -> is_tableau (filter_gtnX_tab n t).
-Proof using .
-  elim: t => [//= | t0 t /= IHt] /and4P [] Hnnil Hrow Hdom Htab.
-  case: (altP ([seq x <- t0 | x <A n] =P [::])) => Ht0 /=; first exact: IHt.
-  rewrite Ht0 /=; apply/and3P; split; last exact: IHt.
-  - apply sorted_filter; last exact Hrow.
-    move=> a b c; exact: leqX_trans.
-  - rewrite (head_filter_gtnX_tab _ Htab).
-    apply filter_gtnX_dominate => //=.
-    move: Htab; by case t => [//= | t1 t'] /= /and3P [].
+Proof using.
+elim: t => [//= | t0 t /= IHt] /and4P [] Hnnil Hrow Hdom Htab.
+case: (altP ([seq x <- t0 | x <A n] =P [::])) => Ht0 /=; first exact: IHt.
+rewrite Ht0 /=; apply/and3P; split; last exact: IHt.
+- apply sorted_filter; last exact Hrow.
+  by move=> a b c; apply: leqX_trans.
+- rewrite (head_filter_gtnX_tab _ Htab).
+  apply filter_gtnX_dominate => //=.
+  by move: Htab; case t => [//= | t1 t'] /= /and3P [].
 Qed.
 
 
 Definition size_tab t := sumn (shape t).
 
 Lemma tab0 t : is_tableau t -> size_tab t = 0 -> t = [::].
-Proof using .
-  move/is_part_sht; rewrite /size_tab => /part0 H/H{H}.
-  rewrite /shape; by case t.
+Proof using.
+move/is_part_sht; rewrite /size_tab => /part0 H/H{H}.
+by rewrite /shape; case t.
 Qed.
 
 Lemma size_to_word t : size (to_word t) = size_tab t.
-Proof using .
-  rewrite /size_tab; elim: t => [//= | t0 t IHt] /=.
-  by rewrite to_word_cons size_cat IHt addnC.
+Proof using.
+rewrite /size_tab; elim: t => [//= | t0 t IHt] /=.
+by rewrite to_word_cons size_cat IHt addnC.
 Qed.
 
 End Tableau.
@@ -466,17 +476,17 @@ Lemma tabsh_readingP (sh : seq nat) (w : seq A) :
   reflect
     (exists tab, [/\ is_tableau tab, shape tab = sh & to_word tab = w])
     (tabsh_reading sh w).
-Proof using .
-  apply (iffP idP).
-  - move=> /andP [] /eqP Hsz Htab.
-    exists (rev (reshape (rev sh) w)); split => //.
-    rewrite shape_rev -{2}(revK sh); congr (rev _).
-    apply: reshapeKl; by rewrite sumn_rev Hsz.
-    rewrite /to_word revK; apply: reshapeKr; by rewrite sumn_rev Hsz.
-  - move=> [] tab [] Htab Hsh Hw; apply/andP; split.
-    + by rewrite -Hw size_to_word /size_tab Hsh.
-    + rewrite -Hw /to_word -Hsh.
-      by rewrite /shape -map_rev -/(shape _) flattenK revK.
+Proof using.
+apply (iffP idP).
+- move=> /andP [] /eqP Hsz Htab.
+  exists (rev (reshape (rev sh) w)); split => //.
+  + rewrite shape_rev -{2}(revK sh); congr (rev _).
+    by apply: reshapeKl; rewrite sumn_rev Hsz.
+  + by rewrite /to_word revK; apply: reshapeKr; rewrite sumn_rev Hsz.
+- move=> [] tab [] Htab Hsh Hw; apply/andP; split.
+  + by rewrite -Hw size_to_word /size_tab Hsh.
+  + rewrite -Hw /to_word -Hsh.
+    by rewrite /shape -map_rev -/(shape _) flattenK revK.
 Qed.
 
 End TableauReading.
@@ -505,36 +515,39 @@ Canonical tabsh_countType := Eval hnf in CountType tabsh tabsh_countMixin.
 Canonical tabsh_subCountType := Eval hnf in [subCountType of tabsh].
 
 Lemma tabshP (t : tabsh) : is_tableau t.
-Proof using . by case: t => t /= /andP []. Qed.
+Proof using. by case: t => t /= /andP []. Qed.
 
 Lemma shape_tabsh (t : tabsh) : shape t = sh.
-Proof using . by case: t => t /= /andP [] _ /eqP. Qed.
+Proof using. by case: t => t /= /andP [] _ /eqP. Qed.
 
 From mathcomp Require Import tuple.
 
 Lemma tabsh_to_wordK (t : tabsh) :
   rev (reshape (rev sh) (to_word (val t))) = t.
-Proof using . rewrite /= -(shape_tabsh t); exact: to_wordK. Qed.
+Proof using. by rewrite /= -(shape_tabsh t); apply: to_wordK. Qed.
 
-Let tabsh_enum : seq tabsh :=
-  pmap insub [seq rev (reshape (rev sh) (val w)) | w in [finType of d.-tuple 'I_n.+1]].
+Let tabsh_enum :
+  seq tabsh :=
+  pmap insub [seq rev (reshape (rev sh) (val w)) |
+              w in [finType of d.-tuple 'I_n.+1]].
+
 Lemma finite_tabsh : Finite.axiom tabsh_enum.
-Proof using .
-  case=> /= t Ht; rewrite -(count_map _ (pred1 t)) (pmap_filter (@insubK _ _ _)).
-  rewrite count_filter -(@eq_count _ (pred1 t)) => [|s /=]; last first.
-    by rewrite isSome_insub; case: eqP=> // ->.
-  move: Ht => /andP [] Htab /eqP Hsh.
-  rewrite count_map.
-  have Htw : size (to_word t) == d.
-    by rewrite size_to_word /size_tab Hsh intpartn_sumn.
-  rewrite (eq_in_count (a2 := pred1 (Tuple Htw))).
-    rewrite enumT; exact: enumP (Tuple Htw).
-  move=> w _ /=; apply/idP/idP.
-  - move=> /eqP Ht; subst t.
-    apply/eqP/val_inj => /=; rewrite /to_word revK.
-    apply esym; apply: reshapeKr; by rewrite sumn_rev size_tuple intpartn_sumn.
-  - move=> /eqP Hw; subst w; rewrite /=.
-    by rewrite /to_word -Hsh -shape_rev flattenK revK.
+Proof using.
+case=> /= t Ht; rewrite -(count_map _ (pred1 t)) (pmap_filter (@insubK _ _ _)).
+rewrite count_filter -(@eq_count _ (pred1 t)) => [|s /=]; last first.
+  by rewrite isSome_insub; case: eqP=> // ->.
+move: Ht => /andP [] Htab /eqP Hsh.
+rewrite count_map.
+have Htw : size (to_word t) == d.
+  by rewrite size_to_word /size_tab Hsh intpartn_sumn.
+rewrite (eq_in_count (a2 := pred1 (Tuple Htw))).
+  by rewrite enumT; apply: enumP (Tuple Htw).
+move=> w _ /=; apply/idP/idP.
+- move=> /eqP Ht; subst t.
+  apply/eqP/val_inj => /=; rewrite /to_word revK.
+  by apply esym; apply: reshapeKr; rewrite sumn_rev size_tuple intpartn_sumn.
+- move=> /eqP Hw; subst w; rewrite /=.
+  by rewrite /to_word -Hsh -shape_rev flattenK revK.
 Qed.
 
 Canonical tabsh_finMixin := Eval hnf in FinMixin finite_tabsh.
@@ -547,30 +560,30 @@ Lemma to_word_enum_tabsh :
     [seq to_word (tabshval t) | t <- enum tabsh]
     [seq x <- [seq val i | i <- enum [finType of d.-tuple 'I_n.+1]]
     | tabsh_reading sh x].
-Proof using .
-  apply uniq_perm_eq.
-  - rewrite map_inj_in_uniq; first exact: enum_uniq.
-    move=> t u _ _ /= Heq; apply val_inj.
-    by rewrite /= -(tabsh_to_wordK t) -(tabsh_to_wordK u) Heq /=.
-  - apply filter_uniq; rewrite map_inj_uniq; last exact: val_inj.
-    exact: enum_uniq.
-  move=> w /=; rewrite /tabsh_reading mem_filter; apply/idP/idP.
-  - move=> /mapP [] t _ -> {w}.
-    rewrite size_to_word /size_tab shape_tabsh eq_refl /=.
-    rewrite tabsh_to_wordK tabshP /=.
-    have Ht : size (to_word (val t)) == d.
-      by rewrite size_to_word /size_tab shape_tabsh intpartn_sumn.
-    have -> : to_word (val t) = val (Tuple Ht) by [].
-    rewrite mem_map; last exact: val_inj.
-    exact: mem_enum.
-  - move=> /andP [] /andP [] /eqP Hsz Htab /mapP [] tpl _ hw; subst w.
-    have Htsh : is_tab_of_shape sh (rev (reshape (rev sh) tpl)).
-      rewrite /is_tab_of_shape /= Htab /= shape_rev reshapeKl ?revK //.
-      by rewrite sumn_rev Hsz.
-    suff -> : val tpl = to_word (TabSh Htsh).
-      apply/mapP; exists (TabSh Htsh) => //; exact: mem_enum.
-    rewrite /= /to_word revK reshapeKr //.
+Proof using.
+apply uniq_perm_eq.
+- rewrite map_inj_in_uniq; first exact: enum_uniq.
+  move=> t u _ _ /= Heq; apply val_inj.
+  by rewrite /= -(tabsh_to_wordK t) -(tabsh_to_wordK u) Heq /=.
+- apply filter_uniq; rewrite map_inj_uniq; last exact: val_inj.
+  exact: enum_uniq.
+move=> w /=; rewrite /tabsh_reading mem_filter; apply/idP/idP.
+- move=> /mapP [] t _ -> {w}.
+  rewrite size_to_word /size_tab shape_tabsh eq_refl /=.
+  rewrite tabsh_to_wordK tabshP /=.
+  have Ht : size (to_word (val t)) == d.
+    by rewrite size_to_word /size_tab shape_tabsh intpartn_sumn.
+  have -> : to_word (val t) = val (Tuple Ht) by [].
+  rewrite mem_map; last exact: val_inj.
+  exact: mem_enum.
+- move=> /andP [] /andP [] /eqP Hsz Htab /mapP [] tpl _ hw; subst w.
+  have Htsh : is_tab_of_shape sh (rev (reshape (rev sh) tpl)).
+    rewrite /is_tab_of_shape /= Htab /= shape_rev reshapeKl ?revK //.
     by rewrite sumn_rev Hsz.
+  suff -> : val tpl = to_word (TabSh Htsh).
+    by apply/mapP; exists (TabSh Htsh) => //; apply: mem_enum.
+  rewrite /= /to_word revK reshapeKr //.
+  by rewrite sumn_rev Hsz.
 Qed.
 
 End FinType.
@@ -619,12 +632,12 @@ apply/is_tableau_getP/is_tableau_getP;
 - have Hrc : is_in_shape (shape t) r c.
     by move: Hrc1; rewrite /is_in_shape => /ltnW.
   rewrite Hndecr; [|exact: mem_to_word | exact: mem_to_word].
-  rewrite -!get_incr_tab //; exact: H2.
+  by rewrite -!get_incr_tab //; apply: H2.
 - have Hrc : is_in_shape (shape t) r c.
     move: Hrc1; rewrite /is_in_shape => /leq_trans; apply.
     by move: H1 => /is_partP [] _; apply.
   rewrite Hincr; [|exact: mem_to_word | exact: mem_to_word].
-  rewrite -!get_incr_tab //; exact: H3.
+  by rewrite -!get_incr_tab //; apply: H3.
 Qed.
 
 End IncrMap.
